progress

sha3/proof/old/MyRO.ec
@@ -1,160 +1,66 @@
-require import Option List FSet NewFMap.
+require import Pair Option List FSet NewFMap.
         import NewLogic Fun.
+require IterProc.
 
-(* TODO: move this *)
-lemma set_eq (m:('a,'b)fmap) x y: m.[x] = Some y => m.[x<-y] = m.
-proof.
-  by rewrite fmapP=> Hx x';rewrite getP;case (x'=x)=>//->;rewrite Hx.
-qed.
-
-lemma oflistK_uniq (s : 'a list) : uniq s =>
-  perm_eq s (elems (oflist s)).
-proof. by move/undup_id => {1}<-; apply/FSet.oflistK. qed.
-
-lemma setD1E (s : 'a fset) x :
-  perm_eq (elems (s `\` fset1 x)) (rem x (elems s)).
-proof.
-rewrite setDE; pose s' := List.filter _ _; apply/(perm_eq_trans s').
-  rewrite perm_eq_sym oflistK_uniq ?filter_uniq ?uniq_elems.
-rewrite /s' rem_filter ?uniq_elems; apply/uniq_perm_eq;
-  rewrite ?filter_uniq ?uniq_elems // => y.
-by rewrite !mem_filter /predC in_fset1.
-qed.
-
-lemma perm_to_rem (s:'a fset) x : 
-  mem s x => perm_eq (elems s) (x :: elems (s `\` fset1 x)).
-proof.
-rewrite memE => /perm_to_rem /perm_eqlP->; apply/perm_cons.
-have /perm_eqlP <- := (setD1E s x); rewrite perm_eq_refl.
-qed.
-
-lemma mem_drop (s:'a list) n x: mem (drop n s) x => mem s x.
-proof. by rewrite -{2}(cat_take_drop n) mem_cat=>->. qed.
-
-lemma mem_take (s:'a list) n x: mem (take n s) x => mem s x.
-proof. by rewrite -{2}(cat_take_drop n) mem_cat=>->. qed.
-(* end TODO *)
-
-abstract theory Titer.
-
-type t.  
-
-module type Orcl = {
-  proc f (x:t) : unit
-}.
-
-module Iter (O:Orcl) = {
-  proc iter(l:t list) = {
-    while (l <> []) { 
-      O.f(head witness l);
-      l <- drop 1 l;
-    }
-  }
-}.
-
-lemma iter_ll(O<:Orcl): islossless O.f => islossless Iter(O).iter.
-proof.
-  move=> O_ll;proc;inline Iter(O).iter.
-  while true (size l);auto=>/=.
-  + call O_ll;skip=> /=?[*]Hl<-;smt ml=0 w=(size_eq0 size_ge0 size_drop).
-  smt ml=0 w=(size_eq0 size_ge0).  
-qed.
-
-section.
-
-declare module O:Orcl.
-
-axiom iter_swap1 i1 i2:  
-  equiv [Iter(O).iter ~ Iter(O).iter :
-         l{1} = [i1;i2] /\ l{2} = [i2;i1] /\ ={glob O} ==> ={glob O}].
-
-lemma iter_swap s1 i s2:
-  equiv [Iter(O).iter ~ Iter(O).iter :
-         l{1} = i::s1++s2 /\ l{2} = s1++i::s2 /\ ={glob O} ==> ={glob O}].
-proof.
-  elim:s1=> /=[|i' s1 Hrec];1:by sim.
-  transitivity Iter(O).iter 
-    (l{1}= i :: i' :: (s1 ++ s2) /\ l{2} = i' :: i :: (s1 ++ s2) /\ ={glob O} ==>
-     ={glob O})
-    (l{1}= i' :: i :: (s1 ++ s2) /\ l{2} = i' :: (s1 ++ i::s2) /\ ={glob O} ==>
-     ={glob O})=>//.
-  + by move=> ?&mr[*]<*>;exists (glob O){mr}, (i' :: i :: (s1 ++ s2)).
-  + proc;rcondt{1}1=>//;rcondt{2}1=>//.
-    rcondt{1}3;1:by auto;conseq(_: true).
-    rcondt{2}3;1:by auto;conseq(_: true).
-    seq 4 4 : (={l,glob O});last by sim.
-    transitivity{1} {Iter(O).iter([i;i']); l <- drop 2 l;} 
-      (l{1} = i :: i' :: (s1 ++ s2) /\ ={l, glob O} ==> ={l,glob O})
-      (l{1} = i :: i' :: (s1 ++ s2) /\ 
-       l{2} = i' :: i :: (s1 ++ s2) /\  ={glob O} ==> ={l,glob O})=>//.
-    + by move=>?&mr[*]<*>;exists (glob O){mr}, (i :: i' :: (s1 ++ s2)).
-    + inline *;rcondt{2} 2;1:by auto. 
-      rcondt{2} 4;1:by auto;sp;conseq(_:true).
-      rcondf{2} 6; auto;call(_:true);wp;call(_:true);auto.
-    transitivity{1} {Iter(O).iter([i';i]); l <- drop 2 l;} 
-      (l{1} = i :: i' :: (s1 ++ s2) /\ 
-       l{2} = i' :: i :: (s1 ++ s2) /\  ={glob O} ==> ={l,glob O})
-      (l{2} = i' :: i :: (s1 ++ s2) /\ ={l, glob O} ==> ={l,glob O})=>//.
-    + by move=>?&mr[*]<*>;exists (glob O){mr}, (i' :: i :: (s1 ++ s2)).
-    + wp; by call (iter_swap1 i i').
-      (* call iter_swap1: FIXME catch exception *)
-    inline *;rcondt{1} 2;1:by auto. 
-    rcondt{1} 4;1:by auto;sp;conseq(_:true).
-    rcondf{1} 6; auto;call(_:true);wp;call(_:true);auto.
-  proc;rcondt{1}1=>//;rcondt{2}1=>//.
-  seq 2 2 : (l{1} = i :: (s1 ++ s2) /\ l{2} = s1 ++ i :: s2 /\ ={glob O}).
-  + by wp;call(_:true);auto;progress;rewrite drop0.
-  transitivity{1} {Iter(O).iter(l); }
-   (={l,glob O} /\ l{1}= i::(s1++s2) ==> ={glob O})
-   (={glob O} /\ l{1}=i::(s1++s2) /\ l{2}= (s1++i::s2) ==> ={glob O})=>//.
-  + by move=>?&mr[*]<*>;exists (glob O){mr}, (i :: (s1 ++ s2)).
-  + by inline *;sim.    
-  transitivity{1} {Iter(O).iter(l); }
-   (={glob O} /\ l{1}=i::(s1++s2) /\ l{2}= (s1++i::s2) ==> ={glob O})
-   (={l,glob O} /\ l{2}= (s1++i::s2) ==> ={glob O})=>//.
-  + by move=>?&mr[*]<*>;exists (glob O){mr}, (s1 ++ i::s2).
-  + by call Hrec;auto.
-  by inline*;sim.         
-qed.
-
-lemma iter_perm : 
-   equiv [Iter(O).iter ~ Iter(O).iter : perm_eq l{1} l{2} /\ ={glob O} ==> ={glob O}].
-proof.
-  exists*l{1},l{2};elim*=>l1 l2;case (perm_eq l1 l2)=> Hp;last first.
-  + conseq (_:false==>_)=>// ??[*]//. 
-  elim: l1 l2 Hp=> [|i s1 ih] s2 eq_s12 /=.
-  + have ->: s2 = [] by apply/perm_eq_small/perm_eq_sym.
-    proc;rcondf{1} 1=>//;rcondf{2} 1=>//.
-  have/perm_eq_mem/(_ i) := eq_s12; rewrite mem_head /=.
-  move/splitPr => [s3 s4] ->>.
-  transitivity Iter(O).iter 
-    (l{1}=i::s1 /\ l{2}=i::(s3++s4) /\ ={glob O} ==> ={glob O})
-    (l{1}=i::(s3++s4) /\ l{2}=s3++i::s4 /\ ={glob O} ==> ={glob O})=>//.
-  + by move=>?&mr[*]-> -> _ ->; exists (glob O){mr}, (i :: (s3 ++ s4)).
-  + proc;rcondt{1}1=>//;rcondt{2}1=>//.
-    seq 2 2: (s1 = l{1} /\ l{2}=s3++s4 /\ ={glob O}).
-    + by wp;call(_:true);auto;progress;rewrite drop0.
-    transitivity{1} {Iter(O).iter(l); }
-      (={l,glob O} ==> ={glob O}) 
-      (s1 = l{1} /\ l{2} = s3 ++ s4 /\ ={glob O} ==> ={glob O})=>//.
-    + by move=>?&mr[*]-> -> ->;exists (glob O){mr}, l{1}.
-    + by inline Iter(O).iter;sim.
-    transitivity{1} {Iter(O).iter(l); }
-      (s1 = l{1} /\ l{2} = s3 ++ s4 /\ ={glob O} ==> ={glob O})
-      (={l,glob O} ==> ={glob O}) =>//.
-    + by move=>?&mr[*]-> -> ->;exists (glob O){mr}, (s3++s4).
-    + move: eq_s12; rewrite -(cat1s i s4) catA perm_eq_sym.
-      rewrite perm_catCA /= perm_cons perm_eq_sym=> Hp.
-    + call (ih (s3++s4) Hp)=>//.
-    by inline Iter(O).iter;sim.
-  by apply (iter_swap s3 i s4). (* FIXME: apply iter_swap fail! *)
-qed.
-
-end section.
-
-end Titer.
+(* FIXME notation *)
+abbrev ([+]) ['a 'b](x : 'b) = fun (_ : 'a) => x.
 
 type flag = [ Unknown | Known ].
+
+lemma neqK_eqU f : f <> Known <=> f = Unknown.
+proof. by case: f. qed.
+
+op in_dom_with (m:('from, 'to * 'flag)fmap) (x:'from) (f:'flag) = 
+   mem (dom m) x /\ (oget (m.[x])).`2 = f.
+
+op restr f (m:('from, 'to * 'flag)fmap) = 
+  let m = filter (fun _ (p:'to*'flag) => p.`2=f) m in
+  map (fun _ (p:'to*'flag) => p.`1) m.
+
+lemma restrP (m:('from, 'to * 'flag)fmap) f x: 
+  (restr f m).[x] = 
+  obind (fun (p:'to*'flag)=>if p.`2=f then Some p.`1 else None) m.[x].
+proof.
+  rewrite /restr /= mapP filterP in_dom /=.
+  by case (m.[x])=>//= -[x0 f'];rewrite oget_some /=;case (f' = f).
+qed.
+
+lemma dom_restr (m:('from, 'to * 'flag)fmap) f x: 
+  mem (dom(restr f m)) x <=> in_dom_with m x f. 
+proof. 
+  rewrite /in_dom_with !in_dom;case: (m.[x]) (restrP m f x)=>//= -[t f'] /=.
+  by rewrite oget_some /=;case (f' = f)=> [_ ->|].
+qed.
+
+lemma restr_set (m:('from, 'to * 'flag)fmap) f1 f2 x y: 
+  restr f1 m.[x<-(y,f2)] = if f1 = f2 then (restr f1 m).[x<-y] else rem x (restr f1 m).
+proof.
+  rewrite fmapP;case (f1=f2)=>[->|Hneq]x0;rewrite !(restrP,getP);1: by case (x0=x).
+  case (x0=x)=>[->|Hnx];1:by rewrite (eq_sym f2) Hneq remP_eq.
+  by rewrite remP Hnx restrP.
+qed.
+
+lemma restr_set_eq (m:('from, 'to * 'flag)fmap) f x y: 
+  restr f m.[x<-(y,f)] = (restr f m).[x<-y].
+proof. by rewrite restr_set. qed.
+
+lemma restr0 f : restr f map0<:'from, 'to * 'flag> = map0.
+proof. by apply fmapP=>x;rewrite restrP !map0P. qed.
+
+lemma restr_set_neq f2 f1 (m:('from, 'to * 'flag)fmap) x y: 
+  !mem (dom m) x =>
+  f2 <> f1 => restr f1 m.[x<-(y,f2)] = restr f1 m.
+proof.
+  by move=>Hm Hneq;rewrite restr_set(eq_sym f1)Hneq rem_id//dom_restr/in_dom_with Hm.
+qed.
+
+lemma restr_rem (m:('from,'to*'flag)fmap) x f: 
+  restr f (rem x m) = 
+   if in_dom_with m x f then rem x (restr f m) else restr f m.
+proof.
+  rewrite fmapP=>z;rewrite restrP;case (in_dom_with m x f);
+   rewrite !(restrP,remP) /in_dom_with in_dom /#.
+qed.
 
 abstract theory Ideal.
 
@@ -166,61 +72,60 @@ module type RO = {
   proc init  ()                  : unit
   proc get   (x : from)          : to
   proc set   (x : from, y : to)  : unit
+  proc rem   (x : from)          : unit
+  proc sample(x : from)          : unit
+}.
+
+module type RO_Distinguisher(G : RO) = {
+  proc distinguish(): bool 
+}.
+
+module type FRO = {
+  proc init  ()                  : unit
+  proc get   (x : from)          : to
+  proc set   (x : from, y : to)  : unit
+  proc rem   (x : from)          : unit 
   proc sample(x : from)          : unit
   proc in_dom(x : from,f : flag) : bool
   proc restrK()                  : (from,to)fmap
 }.
 
-module type Distinguisher(G : RO) = {
+module type FRO_Distinguisher(G : FRO) = {
   proc distinguish(): bool 
 }.
 
-op in_dom_with (m:(from, to * flag)fmap) (x:from) (f:flag) = 
-   mem (dom m) x /\ (oget (m.[x])).`2 = f.
-
-op restr f (m:(from, to * flag)fmap) = 
-  let m = filter (fun _ (p:to*flag) => p.`2=f) m in
-  map (fun _ (p:to*flag) => p.`1) m.
-
-lemma restrP m f x: 
-  (restr f m).[x] = 
-  obind (fun (p:to*flag)=>if p.`2=f then Some p.`1 else None) m.[x].
-proof.
-  rewrite /restr /= mapP filterP in_dom /=.
-  by case (m.[x])=>//= -[x0 f'];rewrite oget_some /=;case (f' = f).
-qed.
-
-lemma restr_dom m f x: 
-  mem (dom(restr f m)) x <=> (mem (dom m) x /\ (oget m.[x]).`2 = f).
-proof. 
-  rewrite !in_dom;case: (m.[x]) (restrP m f x)=>//= -[t f'] /=.
-  by rewrite oget_some /=;case (f' = f)=> [_ ->|].
-qed.
-
-lemma restr_set m f1 f2 x y: 
-  restr f1 m.[x<-(y,f2)] = if f1 = f2 then (restr f1 m).[x<-y] else rem x (restr f1 m).
-proof.
-  rewrite fmapP;case (f1=f2)=>[->|Hneq]x0;rewrite !(restrP,getP);1: by case (x0=x).
-  case (x0=x)=>[->|Hnx];1:by rewrite (eq_sym f2) Hneq remP_eq.
-  by rewrite remP Hnx restrP.
-qed.
-
-lemma restr_set_eq m f x y: 
-  restr f m.[x<-(y,f)] = (restr f m).[x<-y].
-proof. by rewrite restr_set. qed.
-
-lemma restr0 f : restr f map0 = map0.
-proof. by apply fmapP=>x;rewrite restrP !map0P. qed.
-
-lemma restr_set_neq f2 f1 m x y: 
-  !mem (dom m) x =>
-  f2 <> f1 => restr f1 m.[x<-(y,f2)] = restr f1 m.
-proof.
-  by move=>Hm Hneq;rewrite restr_set (eq_sym f1) Hneq rem_id//restr_dom Hm.
-qed.
-
 (* -------------------------------------------------------------------------- *)
 module RO : RO = {
+  var m : (from, to)fmap
+
+  proc init () = { m <- map0; }
+
+  proc get(x:from) = {
+    var r;
+    r <$ sampleto x;
+    if (!mem (dom m) x) m.[x] <- r;
+    return (oget m.[x]);
+  }
+
+  proc set (x:from, y:to) = {
+    m.[x] <- y;
+  }
+
+  proc rem (x:from) = {
+    m <- rem x m;
+  }
+
+  proc sample(x:from) = {
+    get(x);
+  }
+
+  proc restrK() = {
+    return m;
+  }
+
+}.
+
+module FRO : FRO = {
   var m : (from, to * flag)fmap
 
   proc init () = { m <- map0; }
@@ -237,10 +142,14 @@ module RO : RO = {
     m.[x] <- (y,Known);
   }
 
+   proc rem (x:from) = {
+    m <- rem x m;
+  }
+
   proc sample(x:from) = {
     var c;
-    c     <$ sampleto x;
-    m.[x] <- (c,Unknown);
+    c <$ sampleto x;
+    if (!mem (dom m) x) m.[x] <- (c,Unknown);
   }
 
   proc in_dom(x:from, f:flag) = {
@@ -250,323 +159,496 @@ module RO : RO = {
   proc restrK() = {
     return restr Known m;
   }
+
 }.
+
+equiv RO_FRO_init : RO.init ~ FRO.init : true ==> RO.m{1} = map (+fst) FRO.m{2}.
+proof. by proc;auto=>/=;rewrite map_map0. qed.
+
+equiv RO_FRO_get : RO.get ~ FRO.get :
+   ={x} /\ RO.m{1} = map (+fst) FRO.m{2} ==> ={res} /\ RO.m{1} = map (+fst) FRO.m{2}.
+proof. 
+  proc;auto=>?&ml[]->->/=?->/=.
+  rewrite !dom_map !map_set/fst/= getP_eq oget_some;progress.
+  + by rewrite mapP oget_omap_some // -in_dom. 
+  by apply /eq_sym/set_eq;rewrite get_oget?dom_map// mapP oget_omap_some// -in_dom. 
+qed.
+
+equiv RO_FRO_set : RO.set ~ FRO.set :
+   ={x,y} /\ RO.m{1} = map (+fst) FRO.m{2} ==> RO.m{1} = map (+fst) FRO.m{2}.
+proof. by proc;auto=>?&ml[*]3!->;rewrite map_set. qed.
+
+equiv RO_FRO_rem : RO.rem ~ FRO.rem :
+   ={x} /\ RO.m{1} = map (+fst) FRO.m{2} ==> RO.m{1} = map (+fst) FRO.m{2}.
+proof. by proc;auto=>??;rewrite map_rem. qed.
+
+equiv RO_FRO_sample : RO.sample ~ FRO.sample :
+   ={x} /\ RO.m{1} = map (+fst) FRO.m{2} ==> RO.m{1} = map (+fst) FRO.m{2}.
+proof. 
+  by proc;inline *;auto=>?&ml[]2!->/=?->;rewrite dom_map/= map_set. 
+qed.
+
+lemma RO_FRO_D (D<:RO_Distinguisher{RO,FRO}) : 
+  equiv [D(RO).distinguish ~ D(FRO).distinguish : 
+     ={glob D} /\ RO.m{1} = map (+fst) FRO.m{2} ==>
+     ={glob D} /\ RO.m{1} = map (+fst) FRO.m{2} ].
+proof.
+  proc (RO.m{1} = map (+fst) FRO.m{2})=>//.
+  + by conseq RO_FRO_init. + by conseq RO_FRO_get. + by conseq RO_FRO_set. 
+  + by conseq RO_FRO_rem. + by conseq RO_FRO_sample.
+qed.
 
 section LL. 
 
-lemma init_ll : islossless RO.init.
+lemma RO_init_ll : islossless RO.init.
 proof. by proc;auto. qed.
 
-lemma in_dom_ll : islossless RO.in_dom.
+lemma FRO_init_ll : islossless FRO.init.
+proof. by proc;auto. qed.
+
+lemma FRO_in_dom_ll : islossless FRO.in_dom.
 proof. by proc. qed.
 
-lemma restrK_ll : islossless RO.restrK.
+lemma FRO_restrK_ll : islossless FRO.restrK.
 proof. by proc. qed.
 
-lemma set_ll : islossless RO.set.
+lemma RO_set_ll : islossless RO.set.
+proof. by proc;auto. qed.
+
+lemma FRO_set_ll : islossless FRO.set.
 proof. by proc;auto. qed.
 
 axiom sampleto_ll : forall x, Distr.weight (sampleto x) = 1%r.
 
-lemma get_ll : islossless RO.get.
+lemma RO_get_ll : islossless RO.get.
 proof. by proc;auto;progress;apply sampleto_ll. qed.
 
-lemma sample_ll : islossless RO.sample.
+lemma FRO_get_ll : islossless FRO.get.
+proof. by proc;auto;progress;apply sampleto_ll. qed.
+
+lemma RO_sample_ll : islossless RO.sample.
+proof. by proc;call RO_get_ll. qed.
+
+lemma FRO_sample_ll : islossless FRO.sample.
 proof. by proc;auto;progress;apply sampleto_ll. qed.
 
 end section LL.
  
 end Ideal.
 
-
 (* -------------------------------------------------------------------------- *)
+
 abstract theory GenEager.
 
 clone include Ideal. 
 
 axiom sampleto_ll : forall x, Distr.weight (sampleto x) = 1%r.
 
-clone include Titer with type t <- from.
+clone include IterProc with type t <- from.
 
-module ERO : RO = {
+(** A module that resample query if the associate value is unknown *)
+module RRO : FRO = {
 
-  proc init = RO.init
+  proc init = FRO.init
 
   proc get(x:from) = {
     var r;
     r <$ sampleto x;
-    if (!mem (dom RO.m) x || (oget RO.m.[x]).`2 = Unknown) {
-      RO.m.[x] <- (r,Known);
+    if (!mem (dom FRO.m) x || (oget FRO.m.[x]).`2 = Unknown) {
+      FRO.m.[x] <- (r,Known);
     }
-    return (oget RO.m.[x]).`1;
+    return (oget FRO.m.[x]).`1;
   }
 
-  proc set = RO.set 
+  proc set = FRO.set 
 
-  proc sample = RO.sample
+  proc rem = FRO.rem
 
-  proc in_dom = RO.in_dom
+  proc sample = FRO.sample
 
-  proc restrK = RO.restrK
+  proc in_dom = FRO.in_dom
+
+  proc restrK = FRO.restrK
 
   module I = {
-    proc f = sample
+    proc f (x:from) = {
+      var c;
+      c <$ sampleto x;
+      FRO.m.[x] <- (c,Unknown);
+    }
   }
 
   proc resample () = {
-    Iter(I).iter (elems (dom (restr Unknown RO.m)));
+    Iter(I).iter (elems (dom (restr Unknown FRO.m)));
   }
 
 }.
 
-lemma resample_ll : islossless ERO.resample.
+(* A module which is lazy on sample *)
+module LRO : RO = {
+
+  proc init = RO.init
+
+  proc get = RO.get
+
+  proc set = RO.set 
+
+  proc rem = RO.rem
+
+  proc sample(x:from) = {}
+
+}.
+
+lemma RRO_resample_ll : islossless RRO.resample.
 proof. 
-  proc;call (iter_ll ERO.I _)=>//;apply (sample_ll sampleto_ll).
+  proc;call (iter_ll RRO.I _)=>//;proc;auto=>/=?;apply sampleto_ll. 
 qed.
 
 lemma eager_init :
-  eager [ERO.resample(); , RO.init ~ ERO.init, ERO.resample(); :
-         ={RO.m} ==> ={RO.m} ].
+  eager [RRO.resample(); , FRO.init ~ RRO.init, RRO.resample(); :
+         ={FRO.m} ==> ={FRO.m} ].
 proof.
   eager proc. inline{2} *;rcondf{2}3;auto=>/=.
   + by move=>?_;rewrite restr0 dom0 elems_fset0.
-  by conseq (_:) (_:true==>true: =1%r) _=>//;call resample_ll.
+  by conseq (_:) (_:true==>true: =1%r) _=>//;call RRO_resample_ll.
 qed.
 
 lemma iter_perm2 (i1 i2 : from):
-  equiv[ Iter(ERO.I).iter ~ Iter(ERO.I).iter :
-          l{1} = [i1; i2] /\ l{2} = [i2; i1] /\ ={glob ERO.I} ==>
-          ={glob ERO.I}].
+  equiv[ Iter(RRO.I).iter_12 ~ Iter(RRO.I).iter_21 :
+            ={glob RRO.I, t1, t2} ==> ={glob RRO.I}].
 proof.
-  proc;rcondt{1}1=>//;rcondt{2}1=>//.
-  rcondt{1}3;1:by auto;conseq(_:true).
-  rcondt{2}3;1:by auto;conseq(_:true).
-  seq 4 4 : (={l,RO.m});2:by sim.
-  case (i1=i2);1:by sim.
-  inline *;swap[4..5]-2;swap{2} 6-2;auto=>?&mr[*]3!<*>Hneq/=?->?->/=.
-  by rewrite set_set Hneq. 
+  proc;inline *;case ((t1=t2){1});1:by auto.
+  by swap{2}[4..5]-3;auto=> &ml&mr[*]3!->neq/=?->?->;rewrite set_set neq.
 qed.
 
 lemma eager_get :
-  eager [ERO.resample(); , RO.get ~ ERO.get, ERO.resample(); :
-         ={x,RO.m} ==> ={res,RO.m} ].
+  eager [RRO.resample(); , FRO.get ~ RRO.get, RRO.resample(); :
+         ={x,FRO.m} ==> ={res,FRO.m} ].
 proof.
   eager proc.
-  wp;case ((mem (dom RO.m) x /\ (oget RO.m.[x]).`2=Known){1}).
+  wp;case ((mem (dom FRO.m) x /\ (oget FRO.m.[x]).`2=Known){1}).
   + rnd{1};rcondf{2} 2;1:by auto=> /#.
-    alias{1} 1 mx = oget RO.m.[x];inline *.
-    while (={l,RO.m} /\ (!mem l x /\ RO.m.[x] = Some (mx.`1,Known)){1}).
+    exists * ((oget FRO.m.[x{2}]){1}).
+;inline RRO.resample.
+    cut := iter_inv RRO.I (fun z=>x{1}<>z) (fun m1 m2 => m1 = m2 /\ .
+    print iter_inv.
+    while (={l,FRO.m} /\ (!mem l x /\ FRO.m.[x] = Some (mx.`1,Known)){1}).
     + auto=>?&mr[*]-> ->;case (l{mr})=>//=x2 l2 Hmx Hgx?->.
       by rewrite getP drop0 /#.
     auto=>??[*]-> ->/= Hmem HK;rewrite sampleto_ll/==> r _. 
-    rewrite -memE restr_dom Hmem/= HK.
+    rewrite -memE dom_restr Hmem/= HK.
     rewrite {1}get_oget //= -HK;case:(oget _)HK=> x1?/=->.
     by move=>????-> _[*]_-> _ Heq?;rewrite in_dom set_eq Heq. 
   rcondt{2} 2. + auto=> ?[*]-> ->;rewrite negb_and /#.
-  case ((mem (dom RO.m) x){1}).
-  + inline{1} ERO.resample=>/=;rnd{1}.
-    transitivity{1} { Iter(ERO.I).iter(x::elems ((dom (restr Unknown RO.m)) `\` fset1 x));
-                      }
-      (={x,RO.m} /\ mem (dom RO.m{1}) x{1} /\ (oget RO.m{1}.[x{1}]).`2 = Unknown ==>
-       ={x,RO.m})
-      (={x,RO.m} /\ mem (dom RO.m{1}) x{1} /\ (oget RO.m{1}.[x{1}]).`2 = Unknown==>
-       ={x} /\ eq_except RO.m{1} RO.m{2} (fset1 x{1}) /\
-       RO.m{1}.[x{2}] = Some (result{2},Unknown) /\
-       RO.m{2}.[x{2}] = Some (result{2},Known)).
-    + by move=>?&mr[*]-> -> ??;exists RO.m{mr}, x{mr}=>/#.
+  case ((mem (dom FRO.m) x){1}).
+  + inline{1} RRO.resample=>/=;rnd{1}.
+    transitivity{1} 
+      { Iter(RRO.I).iter(x::elems ((dom (restr Unknown FRO.m)) `\` fset1 x)); }
+      (={x,FRO.m} /\ mem (dom FRO.m{1}) x{1} /\ (oget FRO.m{1}.[x{1}]).`2 = Unknown ==>
+       ={x,FRO.m})
+      (={x,FRO.m} /\ mem (dom FRO.m{1}) x{1} /\ (oget FRO.m{1}.[x{1}]).`2 = Unknown==>
+       ={x} /\ eq_except FRO.m{1} FRO.m{2} (fset1 x{1}) /\
+       FRO.m{1}.[x{2}] = Some (result{2},Unknown) /\
+       FRO.m{2}.[x{2}] = Some (result{2},Known)).
+    + by move=>?&mr[*]-> -> ??;exists FRO.m{mr}, x{mr}=>/#.
     + move=>???;rewrite in_dom=>[*]<*>[*]->/eq_except_sym H Hxm Hx2.
       rewrite sampleto_ll=> r _;rewrite /= Hxm oget_some /=;apply /eq_sym.
       have /(congr1 oget):= Hx2 => <-;apply eq_except_set_eq=>//.
       by rewrite in_dom Hx2.
-    + call (iter_perm ERO.I iter_perm2).
+    + call (iter_perm RRO.I iter_perm2).
       skip=> &1 &2 [[->> ->>]] [Hdom Hm];progress.
-      by apply /perm_to_rem/restr_dom;rewrite Hdom Hm.
+      by apply /perm_to_rem/dom_restr;rewrite Hdom Hm.
     inline *;rcondt{1} 2;1:by auto.
     while (={x,l} /\ !mem l{1} x{1}/\
-           eq_except RO.m{1} RO.m{2} (fset1 x{1}) /\
-           RO.m{1}.[x{2}] = Some (result{2}, Unknown) /\
-           RO.m{2}.[x{2}] = Some (result{2}, Known)).
+           eq_except FRO.m{1} FRO.m{2} (fset1 x{1}) /\
+           FRO.m{1}.[x{2}] = Some (result{2}, Unknown) /\
+           FRO.m{2}.[x{2}] = Some (result{2}, Known)).
     + auto=> ?&mr[*]2!->Hm Hex Hm1 Hmr Hneq _/=?->.
-      rewrite (contra _ _ (mem_drop _ 1 _) Hm) /=.
-      rewrite!getP;move:Hm;rewrite-(mem_head_behead witness l{mr})//negb_or=>-[]->_.
-      by rewrite Hm1 Hmr/=;apply eq_except_set. 
+      rewrite (contra _ _ (mem_drop 1 _ _) Hm) /= !getP.
+      move:Hm;rewrite-(mem_head_behead witness l{mr})//negb_or=>-[]-> _/=.
+      rewrite Hm1 Hmr/=;apply eq_except_set=>//.
     auto=>?&mr[[->>->>]][]Hdom Hm /=/=?->/=.
     rewrite !drop0 restr_set /= dom_rem /= -memE !inE /=.
     by rewrite !getP_eq /= oget_some/= set2_eq_except.
   inline *. swap{1}3-2.
-  while (={l,x} /\ !mem l{1} x{1} /\ RO.m{1}.[x{1}] = None /\
-         RO.m{2} = RO.m{1}.[x{2}<-(r{2},Known)]).
+  while (={l,x} /\ !mem l{1} x{1} /\ FRO.m{1}.[x{1}] = None /\
+         FRO.m{2} = FRO.m{1}.[x{2}<-(r{2},Known)]).
   + auto=> ?&mr[*]2!->Hm Hn Heq Hl _/=?->.
-    rewrite (contra _ _ (mem_drop _ 1 _) Hm) /=.
+    rewrite (contra _ _ (mem_drop 1 _ _) Hm) /=.
     rewrite set_set -Heq !getP -(eq_sym (x{mr})).
     by move:Hm;rewrite -(mem_head_behead witness l{mr} Hl) -Hn negb_or=>-[]->.
   auto=> ?&mr[*]2!->_ Hnm/=?->.
-  rewrite -memE restr_set_neq //= restr_dom Hnm /=.
+  rewrite -memE restr_set_neq //= dom_restr Hnm /=.
   by have:=Hnm;rewrite in_dom/==>->/=????->->;rewrite in_dom getP_eq oget_some. 
 qed.
 
 lemma eager_set :
-  eager [ERO.resample(); , RO.set ~ ERO.set, ERO.resample(); :
-         ={x,y} /\ ={RO.m} ==> ={res,RO.m} ].
+  eager [RRO.resample(); , FRO.set ~ RRO.set, RRO.resample(); :
+         ={x,y} /\ ={FRO.m} ==> ={res,FRO.m} ].
 proof.
   eager proc.
-  case ((mem (dom RO.m) x /\ (oget RO.m.[x]).`2 = Unknown){1}).
-  inline{1} ERO.resample=>/=;wp 1 2.
-    transitivity{1} { Iter(ERO.I).iter(x::elems ((dom (restr Unknown RO.m)) `\` fset1 x));
+  case ((mem (dom FRO.m) x /\ (oget FRO.m.[x]).`2 = Unknown){1}).
+  inline{1} RRO.resample=>/=;wp 1 2.
+    transitivity{1} { Iter(RRO.I).iter(x::elems ((dom (restr Unknown FRO.m)) `\` fset1 x));
                       }
-      (={x,y,RO.m} /\ mem (dom RO.m{1}) x{1} /\ (oget RO.m{1}.[x{1}]).`2 = Unknown ==>
-       ={x,y,RO.m})
-      (={x,y,RO.m} /\ mem (dom RO.m{1}) x{1} /\ (oget RO.m{1}.[x{1}]).`2 = Unknown==>
-       ={x,y} /\ eq_except RO.m{1} RO.m{2} (fset1 x{1}) /\
-       RO.m{2}.[x{2}] = Some (y{2},Known)).
-    + by move=>?&mr[*]-> -> ???;exists RO.m{mr}, y{mr}, x{mr}=>/#.
+      (={x,y,FRO.m} /\ mem (dom FRO.m{1}) x{1} /\ (oget FRO.m{1}.[x{1}]).`2 = Unknown ==>
+       ={x,y,FRO.m})
+      (={x,y,FRO.m} /\ mem (dom FRO.m{1}) x{1} /\ (oget FRO.m{1}.[x{1}]).`2 = Unknown==>
+       ={x,y} /\ eq_except FRO.m{1} FRO.m{2} (fset1 x{1}) /\
+       FRO.m{2}.[x{2}] = Some (y{2},Known)).
+    + by move=>?&mr[*]-> -> ???;exists FRO.m{mr}, y{mr}, x{mr}=>/#.
     + move=>??? [*]<*>[*]-> -> Hex Hm2.
-      by rewrite (eq_except_set_eq RO.m{2} RO.m{m} x{2}) ?in_dom ?Hm2// eq_except_sym.
-    + call (iter_perm ERO.I iter_perm2).
+      by rewrite (eq_except_set_eq FRO.m{2} FRO.m{m} x{2}) ?in_dom ?Hm2// eq_except_sym.
+    + call (iter_perm RRO.I iter_perm2).
       skip=>?&mr[][]->>[]->>->>[]Hdom Hm/=.
-      by apply /perm_to_rem/restr_dom;rewrite Hdom Hm.
+      by apply /perm_to_rem/dom_restr;rewrite Hdom Hm.
     inline *;rcondt{1} 2;1:by auto.
     while (={x,l} /\ !mem l{1} x{1}/\
-           eq_except RO.m{1} RO.m{2} (fset1 x{1}) /\
-           RO.m{2}.[x{2}] = Some (y{2}, Known)).
+           eq_except FRO.m{1} FRO.m{2} (fset1 x{1}) /\
+           FRO.m{2}.[x{2}] = Some (y{2}, Known)).
     + auto=> ?&mr[*]2!->Hm Hex Hm1 Hmr _/=?->.
-      rewrite (contra _ _ (mem_drop _ 1 _) Hm) /=.
+      rewrite (contra _ _ (mem_drop 1 _ _) Hm) /=.
       rewrite!getP;move:Hm;rewrite-(mem_head_behead witness l{mr})//negb_or=>-[]->_.
       by rewrite Hm1 /=;apply eq_except_set. 
     auto=>?&mr[*]3!<*>Hdom Hm /=/=;rewrite !drop0 sampleto_ll=>/=?_.
     by rewrite -memE restr_set /= dom_rem !inE !getP_eq set2_eq_except.
   inline *;wp.
   while (={x,l} /\ !mem l{1} x{1}/\
-         eq_except RO.m{1} RO.m{2} (fset1 x{1}) /\
-         RO.m{2}.[x{2}] = Some (y{2}, Known)).
+         eq_except FRO.m{1} FRO.m{2} (fset1 x{1}) /\
+         FRO.m{2}.[x{2}] = Some (y{2}, Known)).
   + auto=> ?&mr[*]2!->Hm Hex Hm1 Hmr _/=?->.
-    rewrite (contra _ _ (mem_drop _ 1 _) Hm) /=.
+    rewrite (contra _ _ (mem_drop 1 _ _) Hm) /=.
     rewrite!getP;move:Hm;rewrite-(mem_head_behead witness l{mr})//negb_or=>-[]->_.
     by rewrite Hm1 /=;apply eq_except_set. 
   auto=> ?&mr[*]3!-> Hnm /=. 
-  rewrite-memE restr_set/=rem_id?restr_dom//=Hnm.
+  rewrite-memE restr_set/=rem_id?dom_restr//=Hnm.
   rewrite getP_eq eq_except_sym set_eq_except/=.
   move=>/=????2!->/=[]/eq_except_sym? Hx2;apply/eq_sym.
   have/(congr1 oget):=Hx2=><-;apply eq_except_set_eq=>//;by rewrite in_dom Hx2.
 qed.
 
+lemma eager_rem: 
+  eager [RRO.resample(); , FRO.rem ~ RRO.rem, RRO.resample(); :
+         ={x} /\ ={FRO.m} ==> ={res,FRO.m} ].
+proof.
+  eager proc;case ((in_dom_with FRO.m x Unknown){1}).
+  + inline RRO.resample;wp.
+    transitivity{1} 
+      { Iter(RRO.I).iter(x::elems (dom (restr Unknown FRO.m) `\` fset1 x)); }
+      (={x,FRO.m}/\(in_dom_with FRO.m x Unknown){1}==> ={x,FRO.m}) 
+      (={x,FRO.m}/\ (in_dom_with FRO.m x Unknown){1} ==> (rem x FRO.m){1} = FRO.m{2})=>//.
+    + by move=>?&mr[*]2!->_;exists FRO.m{mr}, x{mr}.   
+    + call (iter_perm RRO.I iter_perm2);skip=>?&mr[*]2!->?/=.
+      by apply /perm_to_rem/dom_restr. 
+    inline *;rcondt{1}2;1:by auto.
+    while (={l} /\ FRO.m{2} = rem x{1} FRO.m{1} /\ !(mem l x){1}).  
+    + auto=>?&mr[*]->-> ^ + Hm Hl _/=?->.
+      rewrite rem_set-(mem_head_behead witness l{mr})//negb_or=>-[]->_/=.
+      by rewrite (contra _ _ (mem_drop 1 _ _) Hm).
+    auto=>?&mr[*]2!->Hidm/=;rewrite sampleto_ll/==>?.
+    by rewrite drop0 restr_rem Hidm/= dom_rem rem_set -memE !inE.
+  inline *;wp. 
+  while (={l} /\ FRO.m{2} = rem x{1} FRO.m{1} /\ !(mem l x){1}).
+  + auto=>?&mr[*]->-> ^ + Hm Hl _/=?->.
+    rewrite rem_set-(mem_head_behead witness l{mr})//negb_or=>-[]->_/=.
+    by rewrite (contra _ _ (mem_drop 1 _ _) Hm).
+  by auto=>?&mr[*]2!->Hndw/=;rewrite restr_rem Hndw//= -memE dom_restr. 
+qed.
+
 lemma eager_in_dom:
-  eager [ERO.resample(); , RO.in_dom ~ ERO.in_dom, ERO.resample(); :
-         ={x,f} /\ ={RO.m} ==> ={res,RO.m} ].
+  eager [RRO.resample(); , FRO.in_dom ~ RRO.in_dom, RRO.resample(); :
+         ={x,f} /\ ={FRO.m} ==> ={res,FRO.m} ].
 proof.
   eager proc;inline *;wp.
-  while (={l,RO.m} /\ (forall z, mem l z => in_dom_with RO.m z Unknown){1} /\
-         in_dom_with RO.m{1} x{1} f{1} = result{2}).
+  while (={l,FRO.m} /\ (forall z, mem l z => in_dom_with FRO.m z Unknown){1} /\
+         in_dom_with FRO.m{1} x{1} f{1} = result{2}).
   + auto=>?&mr[*]2!->Hz <-?_/=?->/=. 
-    by split=>[z Hm|];rewrite /in_dom_with dom_set getP !inE/#.
-  by auto=>?&mr/=[*]3!->/=;split=>// z;rewrite -memE restr_dom. 
+    split=>[z /mem_drop Hm|];rewrite /in_dom_with dom_set getP !inE /#.
+  by auto=>?&mr/=[*]3!->/=;split=>// z;rewrite -memE dom_restr. 
 qed.
 
 lemma eager_restrK:
-  eager [ERO.resample(); , RO.restrK ~ ERO.restrK, ERO.resample(); :
-         ={RO.m} ==> ={res,RO.m} ].
+  eager [RRO.resample(); , FRO.restrK ~ RRO.restrK, RRO.resample(); :
+         ={FRO.m} ==> ={res,FRO.m} ].
 proof.
   eager proc;inline *;wp.
-  while (={l,RO.m} /\ (forall z, mem l z => in_dom_with RO.m z Unknown){1} /\
-         restr Known RO.m{1} = result{2}).
+  while (={l,FRO.m} /\ (forall z, mem l z => in_dom_with FRO.m z Unknown){1} /\
+         restr Known FRO.m{1} = result{2}).
   + auto=>?&mr[*]2!->Hz<-?_/=?->/=. 
-    split=>[z Hm|];1:by rewrite /in_dom_with dom_set getP !inE/#.
-    rewrite restr_set rem_id?restr_dom//.
+    split=>[z /mem_drop Hm|];1:by rewrite /in_dom_with dom_set getP !inE /#.
+    rewrite restr_set rem_id?dom_restr//.
     by move:H=>/(mem_head_behead witness) /(_ (head witness l{mr})) /= /Hz /#.
-  by auto=>?&mr/=->/=;split=>// z;rewrite -memE restr_dom. 
+  by auto=>?&mr/=->/=;split=>// z;rewrite -memE dom_restr. 
 qed.
 
 lemma eager_sample:
-  eager [ERO.resample(); , RO.sample ~ ERO.sample, ERO.resample(); :
-         ={x,RO.m} ==> ={res,RO.m} ].
+  eager [RRO.resample(); , FRO.sample ~ RRO.sample, RRO.resample(); :
+         ={x,FRO.m} ==> ={res,FRO.m} ].
 proof.
   eager proc.
-  transitivity{2} {
-      c <$ sampleto x; RO.m.[x] <- (c, Unknown);
-      Iter(ERO.I).iter(x::elems ((dom (restr Unknown RO.m)) `\` fset1 x));}
-      (={x,RO.m} ==> ={x,RO.m}) 
-      (={x,RO.m} ==> ={x,RO.m})=>//;last first.
-  + inline{2} ERO.resample;call (iter_perm ERO.I iter_perm2);auto=>?&mr[]->->/=?->.
-    by rewrite !restr_set/= !dom_set perm_eq_sym perm_to_rem !inE.
-  + by move=>?&mr[*]2!->;exists RO.m{mr}, x{mr}.
-  inline ERO.resample;inline{2}*;rcondt{2}4;1:by auto.
-  wp;case ((!mem (dom RO.m) x \/ (oget RO.m.[x]).`2=Known){1}).
-  + inline *;swap{1}3-1.
-    while (={x,l} /\ RO.m{1}.[x{1} <- (c{1}, Unknown)] = RO.m{2} /\ !(mem l x){1}).
-    + auto=>?&mr[*]2!-><- Hnm Hl _/=?->.
-      rewrite (contra _ _ (mem_drop _ 1 _) Hnm) /= set_set.
-      by move:Hnm;rewrite-(mem_head_behead witness l{mr})//negb_or eq_sym=>-[]->.
-    auto=>?&mr[*]2!->?/=;rewrite sampleto_ll=>?_?->;rewrite drop0.
-    rewrite restr_set/= dom_set fsetDK.
-    cut<-/=:dom (restr Unknown RO.m{mr}) =
-            dom (restr Unknown RO.m{mr}) `\` fset1 x{mr}.
-    + apply fsetP=>z;rewrite !(restr_dom,inE)/#.
-    by rewrite set_set/= -memE restr_dom;split=>/#.
-  transitivity{1} {
-    Iter(ERO.I).iter(x::elems ((dom (restr Unknown RO.m)) `\` fset1 x));
-    c<$ sampleto x;}
-    (={x,RO.m} /\ (mem (dom RO.m) x /\ (oget RO.m.[x]).`2=Unknown){1} ==> ={x,c,RO.m}) 
-    (={x,RO.m} /\ (mem (dom RO.m) x /\ (oget RO.m.[x]).`2=Unknown){1} ==> 
-     ={x} /\ RO.m{1}.[x{1} <- (c{1}, Unknown)] = RO.m{2})=>//.
-  + by move=>?&mr[*]2!->?;exists RO.m{mr}, x{mr}=>/#.
-  + rnd;call (iter_perm ERO.I iter_perm2);auto=>?&mr[*]->->/=??;split=>//.
-    by rewrite perm_to_rem restr_dom.
-  inline *;rcondt{1}2;1:by auto.
-  swap{1} 7-2.
-  while (={x,l} /\ RO.m{1}.[x{1} <- (c{1}, Unknown)] = RO.m{2} /\ !(mem l x){1}).
-  + auto=>?&mr[*]2!-><- Hnm Hl _/=?->.
-    rewrite (contra _ _ (mem_drop _ 1 _) Hnm) /= set_set.
-    by move:Hnm;rewrite-(mem_head_behead witness l{mr})//negb_or eq_sym=>-[]->.
-  by auto=>?&mr[*]2!->??/=?->?->;rewrite!drop0 restr_set/=dom_set fsetDK-memE!inE.
+  case (!mem (dom (FRO.m{2})) x{2}).
+  + rcondt{2}2;1:by auto.
+    transitivity{2} {
+      c <$ sampleto x; FRO.m.[x] <- (c, Unknown);
+      Iter(RRO.I).iter(x::elems ((dom (restr Unknown FRO.m)) `\` fset1 x));}
+      (={x,FRO.m} /\ ! mem (dom FRO.m{2}) x{2} ==> ={x,FRO.m}) 
+      (={x,FRO.m} /\ ! mem (dom FRO.m{2}) x{2} ==> ={x,FRO.m})=>//;last first.
+    + inline{2} RRO.resample;call (iter_perm RRO.I iter_perm2);auto=>?&mr[*]2!->?/=?->.
+      by rewrite !restr_set/= !dom_set perm_eq_sym perm_to_rem !inE.
+    + by move=>?&mr[*]2!->?;exists FRO.m{mr}, x{mr}.
+    inline RRO.resample;inline{2}*;rcondt{2}4;1:by auto.
+    inline *;wp;swap{1}-2.
+    while (={l} /\ FRO.m{2} = (FRO.m.[x <- (c,Unknown)]){1} /\
+           (!mem (dom FRO.m) x /\ !mem l x){1}).
+    + auto=>?&mr[*]2!->Hd Hl Hnl _/=?->.
+      rewrite dom_set !inE set_set (contra _ _ (mem_drop 1 _ _) Hl).
+      by move:Hl;rewrite-(mem_head_behead witness l{mr})//negb_or eq_sym=>-[]->.
+    auto=>?&mr[*]2!->Hd;rewrite sampleto_ll=>?_/=?->.
+    rewrite drop0 set_set_eq restr_set/= -memE dom_set fsetDK;split=>//.
+    have^Hx->: !mem (dom (restr Unknown FRO.m{mr})) x{mr} by rewrite dom_restr Hd.
+    cut->//: dom (restr Unknown FRO.m{mr}) `\` fset1 x{mr} =
+             dom (restr Unknown FRO.m{mr}).
+    by rewrite fsetP=>x;rewrite in_fsetD1 /#.
+  rcondf{2}2;1:by auto. 
+  swap{1}2-1;inline*;auto.
+  while (={l,FRO.m} /\ (mem (dom FRO.m) x){1});auto.
+  by move=>?&mr[*]2!->Hm Hl _/=?->;rewrite dom_set !inE Hm.
 qed.
 
 section.
 
-declare module D:Distinguisher {RO}.
+declare module D:FRO_Distinguisher {FRO}.
 
-lemma eager_D : eager [ERO.resample(); , D(RO).distinguish ~ 
-                       D(ERO).distinguish, ERO.resample(); :
-                       ={glob D,RO.m} ==> ={RO.m, glob D} /\ ={res} ].
+lemma eager_D : eager [RRO.resample(); , D(FRO).distinguish ~ 
+                       D(RRO).distinguish, RRO.resample(); :
+                       ={glob D,FRO.m} ==> ={FRO.m, glob D} /\ ={res} ].
 proof.
-  eager proc (H_: ERO.resample(); ~ ERO.resample();: ={RO.m} ==> ={RO.m})
-             (={RO.m})=>//; try by sim.
+  eager proc (H_: RRO.resample(); ~ RRO.resample();: ={FRO.m} ==> ={FRO.m})
+             (={FRO.m})=>//; try by sim.
   + by apply eager_init. + by apply eager_get. + by apply eager_set. 
-  + by apply eager_sample. + by apply eager_in_dom. + by apply eager_restrK. 
+  + by apply eager_rem. + by apply eager_sample. 
+  + by apply eager_in_dom. + by apply eager_restrK. 
 qed.
 
-
-module Eager (D:Distinguisher) = {
+module Eager (D:FRO_Distinguisher) = {
 
   proc main1() = {
     var b;
-    RO.init();
-    b <@ D(RO).distinguish();
+    FRO.init();
+    b <@ D(FRO).distinguish();
     return b;
   }
 
   proc main2() = {
     var b;
-    RO.init();
-    b <@ D(ERO).distinguish();
-    ERO.resample();
+    FRO.init();
+    b <@ D(RRO).distinguish();
+    RRO.resample();
     return b;
   }
 
 }.
 
 equiv Eager_1_2: Eager(D).main1 ~ Eager(D).main2 : 
-  ={glob D} ==> ={res,glob RO, glob D}.
+  ={glob D} ==> ={res,glob FRO, glob D}.
 proof.
   proc.
   transitivity{1} 
-    { RO.init(); ERO.resample(); b <@ D(RO).distinguish(); }
-    (={glob D} ==> ={b,RO.m,glob D})
-    (={glob D} ==> ={b,RO.m,glob D})=> //.
+    { FRO.init(); RRO.resample(); b <@ D(FRO).distinguish(); }
+    (={glob D} ==> ={b,FRO.m,glob D})
+    (={glob D} ==> ={b,FRO.m,glob D})=> //.
   + by move=> ?&mr->;exists (glob D){mr}.
   + inline *;rcondf{2}3;2:by sim.
     by auto=>?;rewrite restr0 dom0 elems_fset0.
-  seq 1 1: (={glob D, RO.m});1:by inline *;auto.
+  seq 1 1: (={glob D, FRO.m});1:by inline *;auto.
   by eager call eager_D. 
 qed.
 
-end GenEager.
+end section.
+
+equiv LRO_RRO_init : LRO.init ~ RRO.init : true ==> RO.m{1} = restr Known FRO.m{2}.
+proof. by proc;auto=>/=;rewrite restr0. qed.
+
+equiv LRO_RRO_get : LRO.get ~ RRO.get :
+   ={x} /\ RO.m{1} = restr Known FRO.m{2} ==> ={res} /\ RO.m{1} = restr Known FRO.m{2}.
+proof. 
+  proc;auto=>?&ml[]->->/=?->/=.
+  rewrite dom_restr negb_and ora_or neqK_eqU.
+  rewrite !restr_set/= !getP_eq oget_some;progress.
+  by move:H;rewrite negb_or/= restrP in_dom /#. 
+qed.
+
+equiv LRO_RRO_set : LRO.set ~ RRO.set :
+   ={x,y} /\ RO.m{1} = restr Known FRO.m{2} ==> RO.m{1} = restr Known FRO.m{2}.
+proof. by proc;auto=>?&ml[*]3!->;rewrite restr_set. qed.
+
+equiv LRO_RRO_rem : LRO.rem ~ RRO.rem :
+   ={x} /\ RO.m{1} = restr Known FRO.m{2} ==> RO.m{1} = restr Known FRO.m{2}.
+proof. 
+  proc;inline *;auto=>?&mr[*]->->. rewrite restr_rem.
+  case (in_dom_with FRO.m{mr} x{mr} Known)=>// Hidw.
+  by rewrite rem_id // dom_restr.
+qed.
+
+equiv LRO_RRO_sample : LRO.sample ~ RRO.sample:
+   ={x} /\ RO.m{1} = restr Known FRO.m{2} ==> RO.m{1} = restr Known FRO.m{2}.
+proof. 
+  proc;auto=>?&ml[]_->;rewrite sampleto_ll=> ??;rewrite restr_set /==>Hnd. 
+  by rewrite rem_id // dom_restr Hnd.
+qed.
+
+lemma LRO_RRO_D (D<:RO_Distinguisher{RO,FRO}) : 
+  equiv [D(LRO).distinguish ~ D(RRO).distinguish : 
+     ={glob D} /\ RO.m{1} = restr Known FRO.m{2} ==>
+     ={glob D} /\ RO.m{1} = restr Known FRO.m{2} ].
+proof.
+  proc (RO.m{1} = restr Known FRO.m{2})=>//.
+  + by conseq LRO_RRO_init. + by conseq LRO_RRO_get. + by conseq LRO_RRO_set.
+  + by conseq LRO_RRO_rem. + by conseq LRO_RRO_sample. 
+qed.
+
+section.
+
+declare module D : RO_Distinguisher{RO,FRO}.
+
+local module M = {
+  proc main1() = {
+    var b;
+    RRO.resample();
+    b <@ D(FRO).distinguish();
+    return b;
+  }
+  
+  proc main2() = {
+    var b;
+    b <@ D(RRO).distinguish();
+    RRO.resample();
+    return b;
+  }
+}.
+
+lemma RO_LRO_D : 
+  equiv [D(RO).distinguish ~ D(LRO).distinguish : 
+     ={glob D,RO.m} ==> ={glob D}].
+proof.
+  transitivity M.main1 
+     (={glob D} /\ FRO.m{2} = map (fun _ c => (c,Known)) RO.m{1} ==>
+        ={glob D})
+     (={glob D} /\ FRO.m{1} = map (fun _ c => (c,Known)) RO.m{2} ==>
+        ={glob D})=>//.
+  + by move=>?&mr[]2!->;exists (glob D){mr},(map(fun _ c =>(c,Known))RO.m{mr}).
+  + proc*;inline M.main1;wp;call (RO_FRO_D D);inline *.
+    rcondf{2}2;auto.
+    + move=> &mr[]_->;apply mem_eq0=>z;rewrite -memE dom_restr mapP dom_map in_dom.
+      by case(RO.m{m}.[_]).
+    by move=>?&mr[]2!->/=;rewrite map_comp map_id.
+  transitivity M.main2
+     (={glob D, FRO.m} ==> ={glob D})
+     (={glob D} /\ FRO.m{1} = map (fun _ c => (c,Known)) RO.m{2} ==>
+        ={glob D})=>//.
+  + by move=>?&mr[]2!->;exists (glob D){mr},(map(fun _ c =>(c,Known))RO.m{mr}).
+  + by proc; eager call (eager_D D);auto.
+  proc*;inline M.main2;wp;call{1} RRO_resample_ll. 
+  symmetry;call (LRO_RRO_D D);auto=> &ml&mr[*]2!->;split=>//=.
+  by rewrite fmapP=>x;rewrite restrP mapP;case (RO.m{ml}.[x]).
+qed.
